compiler/dsl/coq/ReflexQuark.v
@@ -4,6 +4,7 @@ Require Import Reflex.
 Require Import ReflexBase.
 Require Import ReflexDenoted.
 Require Import ReflexFin.
+Require Import ReflexFrontend.
 Require Import ReflexHVec.
 Require Import ReflexVec.
 
@@ -41,22 +42,29 @@ Notation v_t := (None) (only parsing).
 Notation v_s := (Some None) (only parsing).
 Notation v_u := (Some (Some None)) (only parsing).
 
-Inductive COMPT : Type := Tab | Screen | UserInput.
+Inductive COMPT : Set := Tab | Screen | UserInput.
 
-Definition COMPS (t : COMPT) : comp :=
+Definition COMPTDEC : forall (x y : COMPT), decide (x = y).
+Proof. decide equality. Defined.
+
+Definition COMPS (t : COMPT) : compd :=
   match t with
-  | Tab       => mk_comp "Tab"       "test/quark/tab.py"        []
-  | Screen    => mk_comp "Screen"    "test/quark/screen.py"     []
-  | UserInput => mk_comp "UserInput" "test/quark/user-input.py" []
+  | Tab       => mk_compd "Tab"       "test/quark/tab.py"        [] (mk_vdesc [str_d])
+  | Screen    => mk_compd "Screen"    "test/quark/screen.py"     [] (mk_vdesc [])
+  | UserInput => mk_compd "UserInput" "test/quark/user-input.py" [] (mk_vdesc [])
   end.
 
-Definition INIT : init_prog PAYD COMPT KSTD IENVD :=
-  [ fun s => Spawn _ _ _ IENVD Tab       v_t (Logic.eq_refl _)
-  ; fun s => Spawn _ _ _ IENVD Screen    v_s (Logic.eq_refl _)
-  ; fun s => Spawn _ _ _ IENVD UserInput v_u (Logic.eq_refl _)
+Definition default_domain := str_of_string "google.com".
+
+Definition IMSG : msg PAYD := @Build_msg _ PAYD Quit tt.
+
+Definition INIT : init_prog PAYD COMPT COMPS KSTD IMSG IENVD :=
+  [ fun s => Spawn _ _ COMPS _ _ IENVD Tab       (default_domain, tt) None (Logic.eq_refl _)
+  ; fun s => Spawn _ _ COMPS _ _ IENVD Screen    tt                   None (Logic.eq_refl _)
+  ; fun s => Spawn _ _ COMPS _ _ IENVD UserInput tt                   None (Logic.eq_refl _)
   ].
 
-Definition HANDLERS : handlers PAYD COMPT KSTD :=
+Definition HANDLERS : handlers PAYD COMPT COMPS KSTD :=
   (fun m cfd =>
     match tag PAYD m as _tm return
       @sdenote _ SDenoted_vdesc (lkup_tag PAYD _tm) -> _
@@ -64,34 +72,44 @@ Definition HANDLERS : handlers PAYD COMPT KSTD :=
 
     | Input => fun pl =>
        let envd := mk_vdesc [] in
-       existT (fun d => hdlr_prog PAYD COMPT KSTD d) envd (
+       existT (fun d => hdlr_prog PAYD COMPT COMPS KSTD m d) envd (
          let (input, _) := pl in fun st0 =>
-         if fd_eq cfd (shvec_ith (n := projT1 KSTD) _ (projT2 KSTD) (kst _ _ st0) userinput)
+         if fd_eq cfd (shvec_ith (n := projT1 KSTD) _
+                                 (projT2 KSTD) (kst _ _ _ _ st0) userinput)
          then
-           [ fun s => Send PAYD COMPT KSTD envd (StVar KSTD _ curtab) Input (SLit _ _ input, tt) ]
+           [ fun s => Send PAYD COMPT COMPS KSTD _ envd
+                           (StVar _ KSTD m _ curtab) Input
+                           (SLit _ _ m _  input, tt) ]
          else
            []
        )
 
     | Display => fun pl =>
        let envd := mk_vdesc [] in
-       existT (fun d => hdlr_prog PAYD COMPT KSTD d) envd (
+       existT (fun d => hdlr_prog PAYD COMPT COMPS KSTD m d) envd (
          let (url, _) := pl in fun st0 =>
-         if fd_eq cfd (shvec_ith (n := projT1 KSTD) _ (projT2 KSTD) (kst _ _ st0) curtab)
+         if fd_eq cfd (shvec_ith (n := projT1 KSTD) _
+                                 (projT2 KSTD) (kst _ _ _ _ st0) curtab)
          then
-           [ fun s => Send PAYD COMPT KSTD envd (StVar KSTD _ screen) Display (SLit _ _ url, tt) ]
+           [ fun s => Send PAYD COMPT COMPS KSTD _ envd
+                           (StVar _ KSTD m _ screen) Display
+                           (SLit _ _ m _ url, tt) ]
          else
            []
        )
 
     | Quit => fun pl =>
        let envd := mk_vdesc [] in
-       existT (fun d => hdlr_prog PAYD COMPT KSTD d) envd (
+       existT (fun d => hdlr_prog PAYD COMPT COMPS KSTD m d) envd (
          let _ := pl in fun st0 =>
-         if fd_eq cfd (shvec_ith (n := projT1 KSTD) _ (projT2 KSTD) (kst _ _ st0) userinput)
+         if fd_eq
+              cfd
+              (shvec_ith (n := projT1 KSTD) _ (projT2 KSTD) (kst _ _ _ _ st0) userinput)
          then
-           [ fun s => Send PAYD COMPT KSTD envd (StVar KSTD _ curtab) Quit tt
-           ; fun s => Send PAYD COMPT KSTD envd (StVar KSTD _ screen) Quit tt
+           [ fun s => Send PAYD COMPT COMPS KSTD _ envd
+                           (StVar _ KSTD m _ curtab) Quit tt
+           ; fun s => Send PAYD COMPT COMPS KSTD _ envd
+                           (StVar _ KSTD m _ screen) Quit tt
            ]
          else
            []
@@ -102,4 +120,4 @@ Definition HANDLERS : handlers PAYD COMPT KSTD :=
     end (pay PAYD m)
   ).
 
-Definition main := mk_main (Build_spec NB_MSG PAYD IENVD KSTD COMPT COMPS INIT HANDLERS).
+Definition main := mk_main (Build_spec NB_MSG PAYD IENVD KSTD COMPT COMPTDEC COMPS IMSG INIT HANDLERS).
