compiler/dsl/coq/Extract.v
@@ -1,6 +1,7 @@
 Require Import Ynot.Extract.
 Require Import ReflexEcho.
 Require Import ReflexQuark.
+Require Import ReflexSSH.
 
 Extraction Blacklist List String.
 
@@ -15,3 +16,4 @@ Extract Constant ReflexIO.send_fd  => "ReflexImpl.send_fd".
 Cd "../ml".
 Recursive Extraction Library ReflexEcho.
 Recursive Extraction Library ReflexQuark.
+Recursive Extraction Library ReflexSSH.
