compiler/pollang/Tactics.v
@@ -66,17 +66,17 @@ Ltac unpack :=
   | [ Htr : _ = inhabits ?tr |- _ ]
       => match goal with
           (*Valid exchange.*)
-         | [ _ : Reach _ _ _ _ _ _ ?HDLRS _,
+         | [ _ : Reach _ _ _ _ _ _ _ ?HDLRS _,
              H : ?s = _,
-             H' : ?s' = kstate_run_prog _ _ _ _ _ _ ?s _ _,
-             input : kstate_run_prog_return_type _ _ _ _ _ _ _ _ |- _ ]
+             H' : ?s' = kstate_run_prog _ _ _ _ _ _ _ ?s _ _,
+             input : kstate_run_prog_return_type _ _ _ _ _ _ _ _ _ |- _ ]
            => unfold HDLRS in H'; unfold HDLRS in input;
               unfold kstate_run_prog in H'; simpl in *;
               destruct_eq H'; rewrite H in H';
               rewrite H' in Htr; destruct_input input
           (*Initialization.*)
-         | [ s : init_state _ _ _,
-             input : init_state_run_prog_return_type _ _ _ _ _ _ _ _ |- _ ]
+         | [ s : init_state _ _ _ _ _,
+             input : init_state_run_prog_return_type _ _ _ _ _ _ _ _ _ |- _ ]
            => match goal with
               | [ H : s = _ |- _ ]
                 => rewrite H in Htr; destruct_input input
@@ -91,7 +91,7 @@ Ltac clear_useless_hyps :=
            => revert H
          | [ H : _ <> _ |- _ ]
            => revert H
-         | [ H : Reach _ _ _ _ _ _ _ _ |- _ ]
+         | [ H : Reach _ _ _ _ _ _ _ _ _ |- _ ]
            => revert H
          | [ H : In _ _ |- _ ]
            => revert H
@@ -109,12 +109,12 @@ Ltac destruct_unpack :=
 
 Ltac subst_states :=
   repeat match goal with 
-         | [ s : kstate _ _ |- _ ]
+         | [ s : kstate _ _ _ _ |- _ ]
              => match goal with
                 | [ _ : s = _ |- _ ]
                     => subst s
                 end
-         | [ s : init_state _ _ _ |- _ ]
+         | [ s : init_state _ _ _ _ _ |- _ ]
              => match goal with
                 | [ _ : s = _ |- _ ]
                     => subst s
@@ -182,7 +182,7 @@ Ltac act_nmatch :=
 
 Ltac msg_fds_are_ok :=
   match goal with
-  | [ H : ~msg_fds_ok _ _ _ _ |- _ ]
+  | [ H : ~msg_fds_ok _ _ _ _ _ _ |- _ ]
       => contradict H; compute; msg_fds_are_ok
   | [ |- forall i : _, _ ]
       => intro i; destruct_fin i; contradiction || auto
@@ -191,7 +191,7 @@ Ltac msg_fds_are_ok :=
 Ltac reach_induction :=
   intros;
   match goal with
-  | [ _ : ktr _ _ _ = inhabits ?tr, H : Reach _ _ _ _ _ _ _ _ |- _ ]
+  | [ _ : ktr _ _ _ _ _ = inhabits ?tr, H : Reach _ _ _ _ _ _ _ _ _ |- _ ]
       => generalize dependent tr; induction H;
          (*Do not put simpl anywhere in here. It breaks destruct_unpack.*)
          intros; destruct_unpack;
@@ -214,7 +214,7 @@ Ltac impossible :=
 Ltac use_IH_disables :=
   match goal with
   | [ IHReach : context[forall tr' : KTrace _, _],
-      _ : ktr _ _ ?s = inhabits ?tr |- _ ]
+      _ : ktr _ _ _ _ ?s = inhabits ?tr |- _ ]
       => apply IHReach with (tr':=tr); auto (*TODO: auto may not always work here.*)
   end.
 
@@ -234,7 +234,7 @@ Ltac forall_not_disabler s :=
   (*Should this take s as an argument?*)
   reach_induction;
   match goal with
-  | [ H : _ = init_state_run_prog _ _ _ _ _ _ _ _ _,
+  | [ H : _ = init_state_run_prog _ _ _ _ _ _ _ _ _ _,
           H' : context[ List.In ?act _ ] |- _ ]
     => simpl in *; subst_states;
        try solve [impossible]; simpl in H'; decompose [or] H';
@@ -242,7 +242,7 @@ Ltac forall_not_disabler s :=
                  | contradiction]
        (*subst act' works when it is set equal to actual action*)
        (*contradiction works when act' is in nil*)
-  | [ _ : ktr _ _ ?s' = inhabits _, H' : context[ List.In ?act _ ] |- _ ]
+  | [ _ : ktr _ _ _ _ ?s' = inhabits _, H' : context[ List.In ?act _ ] |- _ ]
     => subst_assignments; subst_states; simpl in *;
        try solve [impossible];
        decompose [or] H';
@@ -256,14 +256,20 @@ Ltac match_disables :=
   | [ |- Disables _ _ _ nil ]
       => constructor
   (* Induction hypothesis.*)
-  | [ H : ktr _ _ ?s = inhabits ?tr,
-      IH : forall tr', ktr _ _ ?s = inhabits tr' ->
+  | [ H : ktr _ _ _ _ ?s = inhabits ?tr,
+      IH : forall tr', ktr _ _ _ _ ?s = inhabits tr' ->
                        Disables _ ?past ?future tr'
                        |- Disables _ ?past ?future ?tr ]
       => auto
   (*Branch on whether the head of the trace matches.*)
-  | [ _ : ktr _ _ ?s = inhabits _ |- Disables ?pdv _ ?future (?act::_) ]
-      => let H := fresh "H" in
+  | [ |- Disables ?pdv _ ?future (?act::_) ]
+      => let s := match goal with
+                  | [ _ : ktr _ _ _ _ ?s = inhabits _ |- _ ]
+                      => s
+                  | [ s : init_state _ _ _ _ _ |- _ ]
+                      => s
+                  end in
+         let H := fresh "H" in
          pose proof (decide_act pdv future act) as H;
          destruct H;
          [ contradiction ||
@@ -319,11 +325,11 @@ Ltac exists_past s :=
   (*Should this take s as an argument?*)
   reach_induction;
   match goal with
-  | [ H : _ = init_state_run_prog _ _ _ _ _ _ _ _ _ |- _ ]
+  | [ H : _ = init_state_run_prog _ _ _ _ _ _ _ _ _ _ |- _ ]
     => simpl in *; subst_states;
        try solve [ impossible
                  | releaser_match ]
-  | [ _ : ktr _ _ ?s' = inhabits _ |- _ ]
+  | [ _ : ktr _ _ _ _ ?s' = inhabits _ |- _ ]
     => subst_assignments; subst_states; try subst
        (*For any equalities generated by destructing the action match*);
        simpl in *;
@@ -340,18 +346,24 @@ Ltac match_releases :=
   | [ |- Release _ _ _ nil ]
       => constructor
   (* Induction hypothesis.*)
-  | [ H : ktr _ _ ?s = inhabits ?tr,
-      IH : forall tr', ktr _ _ ?s = inhabits tr' ->
+  | [ H : ktr _ _ _ _ ?s = inhabits ?tr,
+      IH : forall tr', ktr _ _ _ _ ?s = inhabits tr' ->
                        Release _ ?past ?future tr'
                        |- Release _ ?past ?future ?tr ]
       => auto
   (*Branch on whether the head of the trace matches.*)
-  | [ _ : ktr _ _ ?s = inhabits _ |- Release ?pdv _ ?future (?act::_) ]
-      => let H := fresh "H" in
+  | [ |- Release ?pdv _ ?future (?act::_) ]
+      => let s := match goal with
+                  | [ _ : ktr _ _ _ _ ?s = inhabits _ |- _ ]
+                      => s
+                  | [ s : init_state _ _ _ _ _ |- _ ]
+                      => s
+                  end in
+         let H := fresh "H" in
          pose proof (decide_act pdv future act) as H;
          destruct H;
          [ contradiction ||
-           (apply R_future; [ match_releases | exists_past s ])
+           (apply R_future; [ match_releases | try exists_past s ])
          | contradiction ||
            (apply R_not_future; [ match_releases | assumption ]) ]
          (*In some cases, one branch is impossible, so contradiction
@@ -369,8 +381,8 @@ Ltac match_immbefore :=
   | [ |- ImmBefore _ _ _ nil ]
       => constructor
   (*Induction hypothesis*)
-  | [ H : ktr _ _ ?s = inhabits ?tr,
-      IH : forall tr', ktr _ _ ?s = inhabits tr' ->
+  | [ H : ktr _ _ _ _ ?s = inhabits ?tr,
+      IH : forall tr', ktr _ _ _ _ ?s = inhabits tr' ->
                        ImmBefore _ ?oact_b ?oact_a tr'
                        |- ImmBefore _ ?oact_b ?oact_a ?tr ]
       => auto
@@ -396,8 +408,8 @@ Ltac match_immafter :=
   match goal with
   | [ |- ImmAfter _ _ _ nil ]
       => constructor
-  | [ H : ktr _ _ ?s = inhabits ?tr,
-      IH : forall tr', ktr _ _ ?s = inhabits tr' ->
+  | [ H : ktr _ _ _ _ ?s = inhabits ?tr,
+      IH : forall tr', ktr _ _ _ _ ?s = inhabits tr' ->
                        ImmAfter _ ?oact_a ?oact_b tr'
                        |- ImmAfter _ ?oact_a ?oact_b ?tr ]
       => auto
